attacker.v
@@ -5,7 +5,7 @@ From iris.algebra Require Import agree auth csum gset gmap excl namespace_map fr
 From iris.base_logic.lib Require Import auth.
 From iris.heap_lang Require Import notation proofmode metatheory.
 From iris.heap_lang.lib Require Import lock ticket_lock.
-From crypto Require Import lib term crypto primitives tactics.
+From cryptis Require Import lib term cryptis primitives tactics.
 
 Set Implicit Arguments.
 Unset Strict Implicit.
@@ -13,7 +13,7 @@ Unset Printing Implicit Defensive.
 
 Section Attacker.
 
-Context `{!cryptoG Σ, !heapG Σ, !tlockG Σ}.
+Context `{!cryptisG Σ, !heapG Σ, !tlockG Σ}.
 Notation iProp := (iProp Σ).
 
 Implicit Types (v : val) (t : term) (e : expr).
