challenge_response.v
@@ -3,7 +3,7 @@ From mathcomp Require Import ssreflect.
 From iris.algebra Require Import agree auth csum gset gmap excl namespace_map frac.
 From iris.base_logic.lib Require Import auth.
 From iris.heap_lang Require Import notation proofmode.
-From crypto Require Import lib term crypto primitives tactics session.
+From cryptis Require Import lib term cryptis primitives tactics session.
 
 Set Implicit Arguments.
 Unset Strict Implicit.
@@ -20,7 +20,7 @@ A --> B: {nA, nB, vk(B)}_sk(A)
 
 Section CR.
 
-Context `{!heapG Σ, !cryptoG Σ}.
+Context `{!heapG Σ, !cryptisG Σ}.
 Context `{TermMeta Σ term_meta term_meta_token}.
 Notation iProp := (iProp Σ).
 
