session.v
@@ -29,7 +29,7 @@ From mathcomp Require Import ssreflect.
 From iris.algebra Require Import agree auth csum gset gmap excl namespace_map frac.
 From iris.base_logic.lib Require Import auth.
 From iris.heap_lang Require Import notation proofmode.
-From crypto Require Import lib term crypto.
+From cryptis Require Import lib term cryptis.
 
 Set Implicit Arguments.
 Unset Strict Implicit.
@@ -37,7 +37,7 @@ Unset Printing Implicit Defensive.
 
 Section Session.
 
-Context `{!cryptoG Σ, !heapG Σ}.
+Context `{!cryptisG Σ, !heapG Σ}.
 Notation iProp  := (iProp Σ).
 Notation iPropI := (iPropI Σ).
 
